theorems/iN_basic/add.lean
@@ -4,12 +4,22 @@ namespace iN
 
 -- TODO mark not `@[rewrite]` but something for directional equality
 
-@[grind]
+/- @[grind]
 theorem add_comm {n} (x y : iN n)
     : x + y = y + x := by
 
   poison_unroll x y => a b
   simp [iN_unwrap_inst]
+  rw [BitVec.add_comm a b] -/
+
+/- set_option tactic.simp.trace true
+set_option trace.Meta.Tactic.simp true -/
+
+@[grind]
+theorem add_comm {n} (x y : iN n)
+    : x + y <~> y + x := by
+
+  poison_unroll x y => a b
   rw [BitVec.add_comm a b]
 
 @[grind]
@@ -17,7 +27,6 @@ theorem addNsw_comm {n} (x y : iN n)
     : x +nsw y <~> y +nsw x := by
 
   poison_unroll x y => a b
-  simp [iN_unwrap_inst]
   rw [BitVec.saddOverflow_comm a b]
   rw [BitVec.add_comm a b]
 
@@ -26,7 +35,6 @@ theorem addNuw_comm {n} (x y : iN n)
     : x +nuw y <~> y +nuw x := by
 
   poison_unroll x y => a b
-  simp [iN_unwrap_inst]
   rw [BitVec.uaddOverflow_comm a b]
   rw [BitVec.add_comm a b]
 
@@ -35,10 +43,11 @@ theorem addNw_comm {n} (x y : iN n)
     : x +nw y <~> y +nw x := by
 
   poison_unroll x y => a b
-  simp [iN_unwrap_inst]
   rw [BitVec.add_comm a b]
   rw [BitVec.saddOverflow_comm a b]
   rw [BitVec.uaddOverflow_comm a b]
+
+-- TODO adjust goals and hypotheses so you don't need `simp [h, a, b]` everywhere
 
 @[grind]
 theorem addNsw_refine {n} (x y : iN n)
@@ -46,11 +55,10 @@ theorem addNsw_refine {n} (x y : iN n)
 
   poison_unroll x y => a b
 
-  simp [iN_unwrap_inst]
   if h : a.saddOverflow b then
-    simp [h]
+    simp [h, a, b]
   else
-    simp [h]
+    simp [h, a, b]
 
 @[grind]
 theorem addNuw_refine {n} (x y : iN n)
@@ -58,11 +66,10 @@ theorem addNuw_refine {n} (x y : iN n)
 
   poison_unroll x y => a b
 
-  simp [iN_unwrap_inst]
   if h : a.uaddOverflow b then
-    simp [h]
+    simp [h, a, b]
   else
-    simp [h]
+    simp [h, a, b]
 
 @[grind]
 theorem addNw_refine {n} (x y : iN n)
@@ -70,18 +77,16 @@ theorem addNw_refine {n} (x y : iN n)
 
   poison_unroll x y => a b
 
-  simp [iN_unwrap_inst]
   if h1 : (a.saddOverflow b ∨ a.uaddOverflow b) then
-    simp [h1]
+    simp [h1, a, b]
   else
-    simp [h1]
+    simp [h1, a, b]
 
 @[grind]
 theorem add_assoc {n} (x y z : iN n)
     : (x + y) + z = x + (y + z) := by
 
   poison_unroll x y z => a b c
-  simp [iN_unwrap_inst]
   rw [BitVec.add_assoc a b c]
 
 @[grind]
@@ -102,9 +107,13 @@ theorem addNsw_assoc_same_sign {n} {hn : Bits n} (x y z : iN n)
     : (x +nsw y) +nsw z <~> x +nsw (y +nsw z) := by
 
   poison_unroll x y z => a b c
-  simp [iN_unwrap_inst] at *
+  simp [iN_unwrap_inst, iN.poisonWrapper] at *
 
   have h' : a.msb = b.msb ∧ b.msb = c.msb := by
+
+    simp [a, b, c, bitvec, poison, *]
+
+    bv_normalize
     bv_decide
 
   rw [BitVec.saddOverflow_chain_assoc_monotone a b c h']
